Expanded with multiple variables

practice.v
@@ -3,12 +3,15 @@ Require Import Coq.Arith.PeanoNat.
 Require Import Coq.Arith.Even.
 
 Require Import Parity.
+Require Import Maps.
 
-Inductive cexp : Type :=
-  | CNum : nat -> cexp
-  | CVar : cexp
-  | CPlus : cexp -> cexp -> cexp
-  | CMult : cexp -> cexp -> cexp.
+Definition state := total_map nat.
+
+Inductive aexp : Type :=
+  | CNum : nat -> aexp
+  | CVar : string -> aexp
+  | CPlus : aexp -> aexp -> aexp
+  | CMult : aexp -> aexp -> aexp.
 
 (* Find some way to define eval and abstract_eval on the same 
    set of commands; but how then to incorporate that they will
@@ -17,20 +20,20 @@ Inductive cexp : Type :=
    Or have separate expressions like currently implemented, but
    how to estabilish "equivelance" between APlus and CPlus? *)
 
-Fixpoint eval (e : cexp) (x : nat) : nat := 
+Fixpoint eval (st : state) (e : aexp) : nat := 
   match e with
   | CNum n => n
-  | CVar => x
-  | CPlus e1 e2 => eval e1 x + eval e2 x
-  | CMult e1 e2 => eval e1 x * eval e2 x
+  | CVar x => st x
+  | CPlus e1 e2 => eval st e1 + eval st e2
+  | CMult e1 e2 => eval st e1 * eval st e2
   end.
 
-Fixpoint abstract_eval (e : cexp) (p : parity) : parity :=
+Fixpoint abstract_eval (st : state) (e : aexp) : parity :=
   match e with 
   | CNum n => extract n
-  | CVar => p
-  | CPlus p1 p2 => parity_plus (abstract_eval p1 p) (abstract_eval p2 p)
-  | CMult p1 p2 => parity_mult (abstract_eval p1 p) (abstract_eval p2 p)
+  | CVar x => extract (st x)
+  | CPlus p1 p2 => parity_plus (abstract_eval st p1) (abstract_eval st p2)
+  | CMult p1 p2 => parity_mult (abstract_eval st p1) (abstract_eval st p2)
   end.
 
 Inductive isNumber : nat -> Prop :=
@@ -142,33 +145,35 @@ Proof.
   - inversion H.
 Qed.
 
-Lemma abstract_plus_sound : forall e1 e2 p n,
-  gamma (abstract_eval e1 p) (eval e1 n) ->
-  gamma (abstract_eval e2 p) (eval e2 n) ->
-  gamma (abstract_eval (CPlus e1 e2) p) (eval (CPlus e1 e2) n).
+Lemma abstract_plus_sound : forall st e1 e2,
+  gamma (abstract_eval st e1) (eval st e1) ->
+  gamma (abstract_eval st e2) (eval st e2) ->
+  gamma (abstract_eval st (CPlus e1 e2)) (eval st (CPlus e1 e2)).
 Proof.
   intros. simpl. apply gamma_distr_plus; assumption.
 Qed.
 
-Lemma abstract_mult_sound : forall e1 e2 p n,
-  gamma (abstract_eval e1 p) (eval e1 n) ->
-  gamma (abstract_eval e2 p) (eval e2 n) ->
-  gamma (abstract_eval (CMult e1 e2) p) (eval (CMult e1 e2) n).
+Lemma abstract_mult_sound : forall st e1 e2,
+  gamma (abstract_eval st e1) (eval st e1) ->
+  gamma (abstract_eval st e2) (eval st e2) ->
+  gamma (abstract_eval st (CMult e1 e2)) (eval st (CMult e1 e2)).
 Proof. intros. simpl. apply gamma_distr_mult; assumption.
 Qed.
 
-Theorem abstract_eval_sound : forall e p n,
+Theorem abstract_eval_sound : forall st x n p e,
+  st x = n ->
+  extract n = p ->
   (gamma p) n ->
-  (gamma (abstract_eval e p)) (eval e n).
+  (gamma (abstract_eval st e)) (eval st e).
 Proof.
   induction e; intros.
   - (* CNum *)
     simpl. apply gamma_extract_n_n.
   - (* CVar *)
-    simpl. assumption.
+    simpl. apply gamma_extract_n_n.
   - (* CPlus *)
     apply abstract_plus_sound; auto.
-    - (* CMult *)
+  - (* CMult *)
     apply abstract_mult_sound; auto.
 Qed.
 (* proof the equivalance of the galois connection diagram *)
